MathematicalLogic/Notation.lean
@@ -1,32 +1,70 @@
 import Mathlib.Order.Notation
 
+class PropNeg (α : Type u) where
+  neg : α → α
+prefix:58 "~ " => PropNeg.neg
+
+class PropImp (α : Type u) where
+  imp : α → α → α
+infixr:55 (priority := high) " ⇒ " => PropImp.imp
+attribute [match_pattern] PropImp.imp
+
+class PropOr (α : Type u) where
+  or : α → α → α
+infixr:56 " ⩒ " => PropOr.or
+
+class PropAnd (α : Type u) where
+  and : α → α → α
+infixr:57 " ⩑ " => PropAnd.and
+
+class PropIff (α : Type u) where
+  iff : α → α → α
+infix:55 (priority := high) " ⇔ " => PropIff.iff
+
+/-- Typeclass for propositional notations. -/
+class PropNotation (α : Type u) extends Top α, Bot α, PropNeg α, PropImp α, PropOr α, PropAnd α, PropIff α
+
 /--
-  Typeclass for propositional notations. Only `⊥` and `⇒` need to be defined; other notations are derived as follows:
+  For classical logic, only `⊥` and `⇒` need to be defined; other notations are derived as follows:
   - Negation `~ p = p ⇒ ⊥`.
   - True `⊤ = ~ ⊥`.
   - Disjunction (or) `p ⩒ q = ~ p ⇒ q`.
   - Conjunction (and) `p ⩑ q = ~ (p ⇒ ~ q)`.
   - Iff `p ⇔ q = (p ⇒ q) ⩑ (q ⇒ p)`.
  -/
-class PropNotation (α : Type u) where
+class ClassicalPropNotation (α : Type u) where
   false : α
   imp : α → α → α
 
-namespace PropNotation
+namespace ClassicalPropNotation
 
-variable [PropNotation α] (p q : α)
-attribute [match_pattern] imp
+variable {α : Type u} [ClassicalPropNotation α]
 
 instance : Bot α := ⟨false⟩
-infixr:55 (priority := high) " ⇒ " => imp
-def neg (p : α) := p ⇒ ⊥
-prefix:58 "~ " => neg
-instance : Top α := ⟨~ ⊥⟩
-def or (p q : α) := ~ p ⇒ q
-infixr:56 " ⩒ " => or
-def and (p q : α) := ~ (p ⇒ ~ q)
-infixr:57 " ⩑ " => and
-def iff (p q : α) := (p ⇒ q) ⩑ (q ⇒ p)
-infix:55 (priority := high) " ⇔ " => iff
+instance : PropImp α := ⟨imp⟩
 
-end PropNotation
+instance : PropNeg α where
+  neg p := p ⇒ ⊥
+
+instance : Top α where
+  top := ~ ⊥
+
+instance : PropOr α where
+  or p q := ~ p ⇒ q
+
+instance : PropAnd α where
+  and p q := ~ (p ⇒ ~ q)
+
+instance : PropIff α where
+  iff p q := (p ⇒ q) ⩑ (q ⇒ p)
+
+instance : PropNotation α where
+
+variable {p q : α}
+theorem true_def : (⊤ : α) = ~ ⊥ := rfl
+theorem neg_def : ~ p = p ⇒ ⊥ := rfl
+theorem or_def : p ⩒ q = ~ p ⇒ q := rfl
+theorem and_def : p ⩑ q = ~ (p ⇒ ~ q) := rfl
+theorem iff_def : p ⇔ q = (p ⇒ q) ⩑ (q ⇒ p) := rfl
+
+end ClassicalPropNotation
